WIP

src/Index.v
@@ -49,8 +49,8 @@ Definition delete_iindex {T M} (i : index) (f : iindex T M) :
     if Compare_dec.le_lt_dec i j then get_iindex (S j) f V
     else get_iindex j f V.
 
-Definition insert_iindex {T M} (i : index)
-           (a : pnset T M) (f : iindex T M)
+Definition insert_iindex {T M} (a : pnset T M)
+           (i : index) (f : iindex T M)
   : iindex T M :=
   fun V (j : index) =>
     match Compare_dec.lt_eq_lt_dec i j with
@@ -62,7 +62,7 @@ Definition insert_iindex {T M} (i : index)
 (* Derived operations *)
 
 Definition move_iindex {T M} i j (f : iindex T M) :=
-  insert_iindex i (get_iindex j f) (delete_iindex j f).
+  insert_iindex (get_iindex j f) i (delete_iindex j f).
 
 (* Morphism definitions *)
 
@@ -81,7 +81,7 @@ Add Parametric Morphism {T M} : (@delete_iindex T M)
 Qed.
 
 Add Parametric Morphism {T M} : (@insert_iindex T M)
-    with signature eq ==> eq_pnset ==> eq_kmorph ==> eq_kmorph
+    with signature eq_pnset ==> eq ==> eq_kmorph ==> eq_kmorph
       as insert_iindex_mor.
   intros * Heq1 * Heq2 V j; unfold insert_iindex; cbn.
   rewrite Heq1, Heq2, Heq2; easy.
@@ -99,6 +99,220 @@ Qed.
 Definition id_iindex : iindex (knset index) 0 :=
   fun _ (j : index) => j.
 Arguments id_iindex V j /.
+
+(* Reductions *)
+
+Lemma red_delete_iindex_ge {T M} i (f : iindex T M) V j :
+  i <= j ->
+  delete_iindex i f V j = f V (S j).
+Proof.
+  intros; unfold delete_iindex.
+  destruct (le_lt_dec i j); try easy; omega.
+Qed.
+
+Lemma red_delete_iindex_lt {T M} i (f : iindex T M) V j :
+  S j <= i ->
+  delete_iindex i f V j = f V j.
+Proof.
+  intros; unfold delete_iindex.
+  destruct (le_lt_dec i j); try easy; omega.
+Qed.
+
+Lemma red_delete_iindex_same {T M} i (f : iindex T M) V :
+  delete_iindex i f V i = f V (S i).
+Proof.
+  apply red_delete_iindex_ge; auto.
+Qed.
+
+Lemma red_insert_iindex_gt {T M} i a (f : iindex T M) V j :
+  S i <= j ->
+  insert_iindex a i f V j = f V (pred j).
+Proof.
+  intros; unfold insert_iindex.
+  destruct (lt_eq_lt_dec i j) as [[|]|]; try easy; omega.
+Qed.
+
+Lemma red_insert_iindex_eq {T M} i a (f : iindex T M) V j :
+  i = j ->
+  insert_iindex a i f V j = a V.
+Proof.
+  intros; unfold insert_iindex.
+  destruct (lt_eq_lt_dec i j) as [[|]|]; try easy; omega.
+Qed.
+
+Lemma red_insert_iindex_lt {T M} i a (f : iindex T M) V j :
+  S j <= i ->
+  insert_iindex a i f V j = f V j.
+Proof.
+  intros; unfold insert_iindex.
+  destruct (lt_eq_lt_dec i j) as [[|]|]; try easy; omega.
+Qed.
+
+Lemma red_insert_iindex_same {T M} i a (f : iindex T M) V :
+  insert_iindex a i f V i = a V.
+Proof.
+  apply red_insert_iindex_eq; auto.
+Qed.
+
+(* Useful lemma about predecessor and successor *)
+Lemma red_succ_pred i :
+  0 < i ->
+  S (pred i) = i.
+Proof.
+  intros; omega.
+Qed.
+
+Hint Rewrite @red_delete_iindex_same @red_insert_iindex_same
+  : red_iindexs.
+
+Hint Rewrite @red_delete_iindex_ge @red_delete_iindex_lt
+     @red_insert_iindex_gt @red_insert_iindex_eq
+     @red_insert_iindex_lt @red_succ_pred
+     using omega : red_iindexs.
+
+(* Rewrite operations using reductions *)
+Ltac red_iindexs :=
+  autorewrite with red_iindexs in *;
+  repeat progress
+    (try (rewrite_strat topdown (hints red_iindexs)); cbn).
+
+(* Case split on the order of the parameters. *)
+Ltac case_order i j :=
+  destruct (Compare_dec.lt_eq_lt_dec i j) as [[|]|];
+    red_iindexs; [> | replace j with i by easy |]; try omega.
+
+(* Beta and eta rules for [iindex] operations *)
+
+Lemma iindex_beta_get_eq_pointwise {T M} i j a (f : iindex T M) :
+  i = j ->
+  get_iindex i (insert_iindex a j f) =p= a.
+Proof.
+  intros Heq V; red_iindexs; easy.
+Qed.
+
+Definition iindex_beta_get_eq {T M} i j a f :=
+  fun V Heq =>
+    eq_pnset_expand (@iindex_beta_get_eq_pointwise T M i j a f Heq) V.
+
+Lemma iindex_beta_get_pointwise {T M} i a (f : iindex T M) :
+  get_iindex i (insert_iindex a i f) =p= a.
+Proof. apply iindex_beta_get_eq_pointwise; easy. Qed.
+
+Definition iindex_beta_get {T M} i a f :=
+  eq_pnset_expand (@iindex_beta_get_pointwise T M i a f).
+
+Lemma iindex_beta_delete_eq_pointwise {T M} i j a (f : iindex T M) :
+  i = j ->
+  delete_iindex i (insert_iindex a j f) =km= f.
+Proof.
+  intros Heq V k.
+  case_order i k; easy.
+Qed.
+
+Definition iindex_beta_delete_eq {T M} i j a f :=
+  fun V Heq =>
+    eq_kmorph_expand
+      (@iindex_beta_delete_eq_pointwise T M i j a f Heq) V.
+
+Lemma iindex_beta_delete_pointwise {T M} i a (f : iindex T M) :
+  delete_iindex i (insert_iindex a i f) =km= f.
+Proof. apply iindex_beta_delete_eq_pointwise; easy. Qed.
+
+Definition iindex_beta_delete {T M} i a f :=
+  eq_kmorph_expand (@iindex_beta_delete_pointwise T M i a f).
+
+Lemma iindex_eta_eq_pointwise {T M} i j k (f : iindex T M) :
+  i = j ->
+  i = k ->
+  insert_iindex (get_iindex j f) i (delete_iindex k f) =km= f.
+Proof.
+  intros Heq1 Heq2 V l.
+  case_order i l; f_equal; easy.
+Qed.
+
+Definition iindex_eta_eq {T M} i j k f :=
+  fun V Heq1 Heq2 =>
+    eq_kmorph_expand
+      (@iindex_eta_eq_pointwise T M i j k f Heq1 Heq2) V.
+
+Lemma iindex_eta_pointwise {T M} i (f : iindex T M) :
+  insert_iindex (get_iindex i f) i (delete_iindex i f) =km= f.
+Proof. apply iindex_eta_eq_pointwise; easy. Qed.
+
+Definition iindex_eta {T M} i f :=
+  eq_kmorph_expand (@iindex_eta_pointwise T M i f).
+
+Hint Rewrite @iindex_beta_get @iindex_beta_delete @iindex_eta
+  : simpl_iindexs.
+
+Hint Rewrite @iindex_beta_get_eq @iindex_beta_delete_eq @iindex_eta_eq
+  using omega : simpl_iindexs_eqn.
+
+Hint Rewrite @iindex_beta_get_pointwise
+     @iindex_beta_delete_pointwise @iindex_eta_pointwise
+  : simpl_iindexs_pointwise.
+
+Hint Rewrite @iindex_beta_get_eq_pointwise
+     @iindex_beta_delete_eq_pointwise
+     @iindex_eta_eq_pointwise
+  using omega : simpl_iindexs_pointwise_eqn.
+
+(* Unfolding derived operations *)
+
+Lemma unfold_move_iindex {T M} i j (f : iindex T M) :
+  move_iindex i j f =
+  insert_iindex (get_iindex j f) i (delete_iindex j f).
+Proof. easy. Qed.
+
+Hint Rewrite @unfold_move_iindex : unfold_iindexs.
+
+(* Folding derived operations *)
+
+Lemma fold_move_iindex {T M} i j (f : iindex T M) :
+  insert_iindex (get_iindex j f) i (delete_iindex j f)
+  = move_iindex i j f.
+Proof. easy. Qed.
+
+Hint Rewrite @fold_move_iindex : fold_iindexs.
+
+(* Simplify [iindex] terms by unfolding, simplifying and folding *)
+Ltac simpl_iindexs :=
+  autorewrite with unfold_iindexs;
+  autorewrite with simpl_indexs simpl_iindexs;
+  repeat progress
+    (cbn;
+     try (rewrite_strat topdown (hints simpl_indexs));
+     try (rewrite_strat topdown (hints simpl_iindexs)));
+  autorewrite with fold_iindexs.
+
+Ltac simpl_iindexs_eqn :=
+  autorewrite with unfold_iindexs;
+  autorewrite with simpl_indexs simpl_iindexs;
+  repeat progress
+    (cbn;
+     try (rewrite_strat topdown (hints simpl_indexs));
+     try (rewrite_strat topdown (hints simpl_iindexs));
+     try (rewrite_strat topdown (hints simpl_iindexs_eqn)));
+  autorewrite with fold_iindexs.
+
+Ltac simpl_iindexs_pointwise :=
+  autorewrite with unfold_iindexs;
+  autorewrite with simpl_indexs simpl_iindexs_pointwise;
+  repeat progress
+    (cbn;
+     try (rewrite_strat topdown (hints simpl_indexs));
+     try (rewrite_strat topdown (hints simpl_iindexs_pointwise)));
+  autorewrite with fold_iindexs.
+
+Ltac simpl_iindexs_pointwise_eqn :=
+  autorewrite with unfold_iindexs;
+  autorewrite with simpl_indexs simpl_iindexs_pointwise;
+  repeat progress
+    (cbn;
+     try (rewrite_strat topdown (hints simpl_indexs));
+     try (rewrite_strat topdown (hints simpl_iindexs_pointwise));
+     try (rewrite_strat topdown (hints simpl_iindexs_pointwise_eqn)));
+  autorewrite with fold_iindexs.
 
 (* Operational transforms
 
@@ -143,74 +357,36 @@ Arguments id_iindex V j /.
 *)
 
 Definition shift_index (i : index) : index -> index :=
-  delete_iindex i id_iindex 0.
+  fun (j : index) =>
+    if Compare_dec.le_lt_dec i j then S j
+    else j.
 
 Definition unshift_index (i : index) : index -> index :=
-  insert_iindex i (pnset_const i) id_iindex 0.
+  fun (j : index) =>
+    if Compare_dec.le_lt_dec j i then j
+    else pred j.
 
 Definition shift_above_index (i : index) : index -> index :=
   shift_index (S i).
 
+Definition contract_down_index (i : index) : index -> index :=
+  fun (j : index) =>
+    if Nat.eq_dec (S i) j then i
+    else j.
+
+Definition contract_up_index (i : index) : index -> index :=
+  fun (j : index) =>
+    if Nat.eq_dec i (S j) then i
+    else j.
+
 (* Reductions *)
-
-Lemma red_delete_iindex_ge {T M} i (f : iindex T M) V j :
-  i <= j ->
-  delete_iindex i f V j = f V (S j).
-Proof.
-  intros; unfold delete_iindex.
-  destruct (le_lt_dec i j); try easy; omega.
-Qed.
-
-Lemma red_delete_iindex_lt {T M} i (f : iindex T M) V j :
-  S j <= i ->
-  delete_iindex i f V j = f V j.
-Proof.
-  intros; unfold delete_iindex.
-  destruct (le_lt_dec i j); try easy; omega.
-Qed.
-
-Lemma red_delete_iindex_same {T M} i (f : iindex T M) V :
-  delete_iindex i f V i = f V (S i).
-Proof.
-  apply red_delete_iindex_ge; auto.
-Qed.
-
-Lemma red_insert_iindex_gt {T M} i a (f : iindex T M) V j :
-  S i <= j ->
-  insert_iindex i a f V j = f V (pred j).
-Proof.
-  intros; unfold insert_iindex.
-  destruct (lt_eq_lt_dec i j) as [[|]|]; try easy; omega.
-Qed.
-
-Lemma red_insert_iindex_eq {T M} i a (f : iindex T M) V j :
-  i = j ->
-  insert_iindex i a f V j = a V.
-Proof.
-  intros; unfold insert_iindex.
-  destruct (lt_eq_lt_dec i j) as [[|]|]; try easy; omega.
-Qed.
-
-Lemma red_insert_iindex_lt {T M} i a (f : iindex T M) V j :
-  S j <= i ->
-  insert_iindex i a f V j = f V j.
-Proof.
-  intros; unfold insert_iindex.
-  destruct (lt_eq_lt_dec i j) as [[|]|]; try easy; omega.
-Qed.
-
-Lemma red_insert_iindex_same {T M} i a (f : iindex T M) V :
-  insert_iindex i a f V i = a V.
-Proof.
-  apply red_insert_iindex_eq; auto.
-Qed.
 
 Lemma red_shift_index_ge i j :
   i <= j ->
   shift_index i j = S j.
 Proof.
   intros; unfold shift_index.
-  rewrite red_delete_iindex_ge by easy; easy.
+  destruct (le_lt_dec i j); try easy; omega.
 Qed.
 
 Lemma red_shift_index_lt i j :
@@ -218,7 +394,7 @@ Lemma red_shift_index_lt i j :
   shift_index i j = j.
 Proof.
   intros; unfold shift_index.
-  rewrite red_delete_iindex_lt by easy; easy.
+  destruct (le_lt_dec i j); try easy; omega.
 Qed.
 
 Lemma red_shift_index_same i :
@@ -232,17 +408,15 @@ Lemma red_unshift_index_gt i j :
   unshift_index i j = pred j.
 Proof.
   intros; unfold unshift_index.
-  rewrite red_insert_iindex_gt by easy; easy.
+  destruct (le_lt_dec j i); try easy; omega.
 Qed.
 
 Lemma red_unshift_index_le i j :
   j <= i ->
   unshift_index i j = j.
 Proof.
-  intros Hle; unfold unshift_index.
-  destruct (le_lt_eq_dec j i Hle).
-  - rewrite red_insert_iindex_lt by easy; easy.
-  - rewrite red_insert_iindex_eq by easy; easy.
+  intros; unfold unshift_index.
+  destruct (le_lt_dec j i); try easy; omega.
 Qed.
 
 Lemma red_unshift_index_same i :
@@ -273,142 +447,256 @@ Proof.
   apply red_shift_above_index_le; omega.
 Qed.
 
-Lemma red_move_iindex_eq {T M} i j (f : iindex T M) V k :
-  i = k ->
-  move_iindex i j f V k = get_iindex j f V.
+Lemma red_contract_down_index_neq i j :
+  j <> S i ->
+  contract_down_index i j = j.
 Proof.
-  intros; unfold move_iindex.
-  rewrite red_insert_iindex_eq by easy; easy.
+  intros; unfold contract_down_index.
+  destruct (Nat.eq_dec (S i) j); omega.
 Qed.
 
-Lemma red_move_iindex_neq {T M} i j (f : iindex T M) V k :
-  i <> k ->
-  move_iindex i j f V k = delete_iindex j f V (unshift_index i k).
+Lemma red_contract_down_index_eq i j :
+  j = S i ->
+  contract_down_index i j = i.
 Proof.
-  intros; unfold move_iindex.
-  destruct (lt_eq_lt_dec i k) as [[|]|]; try omega.
-  - rewrite red_insert_iindex_gt by easy.
-    rewrite red_unshift_index_gt by easy.
-    easy.
-  - rewrite red_insert_iindex_lt by easy.
-    rewrite red_unshift_index_le by omega.
-    easy.
+  intros; unfold contract_down_index.
+  destruct (Nat.eq_dec (S i) j); omega.
 Qed.
 
-Lemma red_move_iindex_same {T M} i j (f : iindex T M) V :
-  move_iindex i j f V i = get_iindex j f V.
+Lemma red_contract_down_index_same i :
+  contract_down_index i i = i.
 Proof.
-  intros; unfold move_iindex.
-  rewrite red_insert_iindex_same by easy; easy.
+  apply red_contract_down_index_neq; omega.
 Qed.
 
-(* Useful lemma about predecessor and successor *)
-Lemma red_succ_pred i :
-  0 < i ->
-  S (pred i) = i.
+Lemma red_contract_up_index_neq i j :
+  S j <> i ->
+  contract_up_index i j = j.
 Proof.
-  intros; omega.
+  intros; unfold contract_up_index.
+  destruct (Nat.eq_dec i (S j)); omega.
 Qed.
 
-Hint Rewrite @red_delete_iindex_same @red_insert_iindex_same
-     @red_move_iindex_same @red_shift_index_same
-     @red_unshift_index_same @red_shift_above_index_same
+Lemma red_contract_up_index_eq i j :
+  S j = i ->
+  contract_up_index i j = i.
+Proof.
+  intros; unfold contract_up_index.
+  destruct (Nat.eq_dec i (S j)); omega.
+Qed.
+
+Lemma red_contract_up_index_same i :
+  contract_up_index i i = i.
+Proof.
+  apply red_contract_up_index_neq; omega.
+Qed.
+
+Hint Rewrite @red_shift_index_same @red_unshift_index_same
+     @red_shift_above_index_same @red_contract_down_index_same
+     @red_contract_up_index_same
   : red_iindexs.
 
-Hint Rewrite @red_delete_iindex_ge @red_delete_iindex_lt
-     @red_insert_iindex_gt @red_insert_iindex_eq
-     @red_insert_iindex_lt @red_move_iindex_eq @red_move_iindex_neq
-     @red_shift_index_ge @red_shift_index_lt @red_unshift_index_le
-     @red_unshift_index_gt @red_shift_above_index_le
-     @red_shift_above_index_gt @red_succ_pred
+Hint Rewrite @red_shift_index_ge @red_shift_index_lt
+     @red_unshift_index_le @red_unshift_index_gt
+     @red_shift_above_index_le @red_shift_above_index_gt
+     @red_contract_down_index_neq @red_contract_down_index_eq
+     @red_contract_up_index_neq @red_contract_up_index_eq
      using omega : red_iindexs.
 
-(* Rewrite operations using reductions *)
-Ltac red_iindexs :=
-  autorewrite with red_iindexs;
-  repeat progress
-    (try (rewrite_strat topdown (hints red_iindexs)); cbn).
+(* Useful lemmas about shifting *)
 
-(* Case split on the order of the parameters. *)
-Ltac case_order i j :=
-  destruct (Compare_dec.lt_eq_lt_dec i j) as [[|]|];
-    red_iindexs; [> | replace j with i by easy |]; try omega.
-
-(* Beta and eta rules for [iindex] operations *)
-
-Lemma iindex_beta_get_eq_pointwise {T M} i j a (f : iindex T M) :
-  i = j ->
-  get_iindex i (insert_iindex j a f) =p= a.
+Lemma shift_index_neq i j :
+  shift_index i j <> i.
 Proof.
-  intros Heq V; red_iindexs; easy.
+  case_order i j; omega.
 Qed.
 
-Definition iindex_beta_get_eq {T M} i j a f :=
-  fun V Heq =>
-    eq_pnset_expand (@iindex_beta_get_eq_pointwise T M i j a f Heq) V.
-
-Lemma iindex_beta_get_pointwise {T M} i a (f : iindex T M) :
-  get_iindex i (insert_iindex i a f) =p= a.
-Proof. apply iindex_beta_get_eq_pointwise; easy. Qed.
-
-Definition iindex_beta_get {T M} i a f :=
-  eq_pnset_expand (@iindex_beta_get_pointwise T M i a f).
-
-Lemma iindex_beta_delete_eq_pointwise {T M} i j a (f : iindex T M) :
-  i = j ->
-  delete_iindex i (insert_iindex j a f) =km= f.
+Lemma shift_above_index_neq_shift_index i j :
+  shift_above_index i j <> shift_index j i.
 Proof.
-  intros Heq V k.
-  case_order i k; easy.
+  case_order i j; omega.
 Qed.
 
-Definition iindex_beta_delete_eq {T M} i j a f :=
-  fun V Heq =>
-    eq_kmorph_expand
-      (@iindex_beta_delete_eq_pointwise T M i j a f Heq) V.
+Inductive iindex_op T M : Type :=
+  | Ins : pnset T M -> iindex_op T M
+  | Del : iindex_op T M.
+Arguments Ins {T M} a.
+Arguments Del {T M}.
 
-Lemma iindex_beta_delete_pointwise {T M} i a (f : iindex T M) :
-  delete_iindex i (insert_iindex i a f) =km= f.
-Proof. apply iindex_beta_delete_eq_pointwise; easy. Qed.
+Definition apply_iindex_op {T M}
+           (op : iindex_op T M) :=
+  match op with
+  | Ins a => insert_iindex a
+  | Del => delete_iindex
+  end.
 
-Definition iindex_beta_delete {T M} i a f :=
-  eq_kmorph_expand (@iindex_beta_delete_pointwise T M i a f).
+Definition normalize_iindex_left {T M} (op1 op2 : iindex_op T M)
+  : index -> index -> index :=
+  match op1, op2 with
+  | Ins _, Ins _ => fun i1 i2 => i1
+  | Ins _, Del => fun i1 i2 => i1
+  | Del, Ins _ => fun i1 i2 => contract_down_index i2 i1
+  | Del, Del => fun i1 i2 => i1
+  end.
 
-Lemma iindex_eta_eq_pointwise {T M} i j k (f : iindex T M) :
-  i = j ->
-  i = k ->
-  insert_iindex i (get_iindex j f) (delete_iindex k f) =km= f.
+Definition normalize_iindex_right {T M} (op1 op2 : iindex_op T M) :=
+  match op1, op2 with
+  | Ins _, Ins _ => fun i1 i2 => i2
+  | Ins _, Del => fun i1 i2 => i2
+  | Del, Ins _ => fun i1 i2 => contract_up_index i1 i2
+  | Del, Del => fun i1 i2 => i2
+  end.
+
+Lemma normalize_iindex {T M} (op1 op2 : iindex_op T M) :
+  forall i1 i2 f,
+    apply_iindex_op op1 i1
+      (apply_iindex_op op2 i2 f)
+    =km= apply_iindex_op op1 (normalize_iindex_left op1 op2 i1 i2)
+           (apply_iindex_op op2 (normalize_iindex_right op1 op2 i1 i2) f).
 Proof.
-  intros Heq1 Heq2 V l.
-  case_order i l; f_equal; easy.
+  intros i1 i2 f.
+  destruct op1, op2; cbn; try easy.
+  case_order i1 (S i2); try easy; subst.
+  intros V i3.
+  case_order i2 i3; easy.
 Qed.
 
-Definition iindex_eta_eq {T M} i j k f :=
-  fun V Heq1 Heq2 =>
-    eq_kmorph_expand
-      (@iindex_eta_eq_pointwise T M i j k f Heq1 Heq2) V.
+Definition transpose_iindex_left {T M} (op1 op2 : iindex_op T M) :=
+  match op1, op2 with
+  | Ins _, Ins _ => shift_index
+  | Del, Ins _ => unshift_index
+  | Ins _, Del => shift_above_index
+  | Del, Del => unshift_index
+  end.
+Arguments transpose_iindex_left {T M} !op1 !op2.
 
-Lemma iindex_eta_pointwise {T M} i (f : iindex T M) :
-  insert_iindex i (get_iindex i f) (delete_iindex i f) =km= f.
-Proof. apply iindex_eta_eq_pointwise; easy. Qed.
+Definition transpose_iindex_right {T M} (op1 op2 : iindex_op T M) :=
+  match op1, op2 with
+  | Ins _, Ins _ => fun i1 i2 => unshift_index i2 i1
+  | Ins _, Del => fun i1 i2 => shift_index i2 i1
+  | Del, Ins _ => fun i1 i2 => unshift_index i2 i1
+  | Del, Del => fun i1 i2 => shift_index i2 i1
+  end.
+Arguments transpose_iindex_right {T M} !op1 !op2.
 
-Definition iindex_eta {T M} i f :=
-  eq_kmorph_expand (@iindex_eta_pointwise T M i f).
+Definition irreducible_iindex_ops {T M} (op1 op2 : iindex_op T M)
+  : index -> index -> Prop :=
+  match op1, op2 with
+  | Ins _, Ins _ => fun i1 i2 => True
+  | Ins _, Del => fun i1 i2 => True
+  | Del, Ins _ => fun i1 i2 => i1 <> i2
+  | Del, Del => fun i1 i2 => True
+  end.
 
-Hint Rewrite @iindex_beta_get @iindex_beta_delete @iindex_eta
-  : simpl_iindexs.
+Lemma transpose_iindex {T M} (op1 op2 : iindex_op T M) :
+  forall i1 i2 f,
+    irreducible_iindex_ops op1 op2 i1 i2 ->
+    apply_iindex_op op1 i1
+      (apply_iindex_op op2 i2 f)
+    =km= apply_iindex_op op2 (transpose_iindex_left op1 op2 i1 i2)
+          (apply_iindex_op op1 (transpose_iindex_right op1 op2 i1 i2) f).
+Proof.
+  intros i1 i2 f Hirr V i3.
+  destruct op1, op2; cbn;
+    case_order i1 i2;
+      case_order i2 i3; try easy;
+        case_order i1 i3; try easy.
+  - case_order i2 (pred i3); easy.
+  - case_order i2 (pred i3); easy.
+  - case_order i2 (S i3); easy.
+  - case_order i2 (S i1); easy.
+  - case_order i2 (S i3); easy.
+  - case_order i2 (S i1); easy.
+Qed.
 
-Hint Rewrite @iindex_beta_get_eq @iindex_beta_delete_eq @iindex_eta_eq
-  using omega : simpl_iindexs_eqn.
+Lemma transpose_iindex_squared_left {T M} (op1 op2 : iindex_op T M) :
+  forall i1 i2,
+    transpose_iindex_left op2 op1
+      (transpose_iindex_left op1 op2 i1 i2)
+      (transpose_iindex_right op1 op2 i1 i2)
+    = normalize_iindex_left op1 op2 i1 i2.
+Proof.
+  intros.
+  destruct op1, op2; cbn;
+    case_order i1 i2.
+  case_order i2 (pred i1).
+Qed.
 
-Hint Rewrite @iindex_beta_get_pointwise
-     @iindex_beta_delete_pointwise @iindex_eta_pointwise
-  : simpl_iindexs_pointwise.
+Lemma transpose_iindex_squared_right {T M} (op1 op2 : iindex_op T M) :
+  forall i1 i2,
+    irreducible_iindex_ops op1 op2 i1 i2 ->
+    transpose_iindex_right op2 op1
+      (transpose_iindex_left op1 op2 i1 i2)
+      (transpose_iindex_right op1 op2 i1 i2)
+    = normalize_iindex_right op1 op2 i1 i2.
+Proof.
+  intros i1 i2 Hirr.
+  destruct op1, op2; cbn in Hirr |- *;
+    case_order i1 i2.
+  case_order i2 (pred i1).
+Qed.
 
-Hint Rewrite @iindex_beta_get_eq_pointwise
-     @iindex_beta_delete_eq_pointwise
-     @iindex_eta_eq_pointwise
-  using omega : simpl_iindexs_pointwise_eqn.
+Lemma transpose_iindex_reverse_left  {T M} (op1 op2 op3 : iindex_op T M) :
+  forall i1 i2 i3,
+    irreducible_iindex_ops op1 op2 i1 i2 ->
+    irreducible_iindex_ops op2 op3 i2 i3 ->
+    irreducible_iindex_ops op1 op3 i1 (transpose_iindex_left op2 op3 i2 i3) ->
+    transpose_iindex_left op2 op3 (transpose_iindex_left op1 op2 i1 i2)
+      (transpose_iindex_left op1 op3
+         (transpose_iindex_right op1 op2 i1 i2) i3)
+    = normalize_iindex_left op3 op2
+        (transpose_iindex_left op1 op3 i1
+          (transpose_iindex_left op2 op3 i2 i3))
+        (transpose_iindex_left op1 op2 i1 i2).
+Proof.
+  intros i1 i2 i3 Hirr1 Hirr2 Hirr3.
+  remember op1 as oper1.
+  remember op2 as oper2.
+  remember op3 as oper3.
+  destruct oper1, oper2, oper3; cbn in *;
+    case_order i1 i2;
+      case_order i2 i3; try easy;
+        case_order i1 i3; try easy.
+  - case_order i3 (pred i1).
+  - case_order i2 (pred i1).
+  - case_order i1 (pred i3).
+  - case_order i1 (pred i3).
+  - case_order i2 (pred i3).
+  - case_order i1 (pred i3).
+  - case_order i1 (pred i3).
+Qed.
+
+Lemma transpose_iindex_reverse_right  {T M} (op1 op2 op3 : iindex_op T M) :
+  forall i1 i2 i3,
+(*    irreducible_iindex_ops op1 op2 i1 i2 ->
+    irreducible_iindex_ops op2 op3 i2 i3 ->
+    irreducible_iindex_ops op1 op3 i1 (transpose_iindex_left op2 op3 i2 i3) ->*)
+    transpose_iindex_right op1 op2
+      (transpose_iindex_right op1 op3 i1
+         (transpose_iindex_left op2 op3 i2 i3))
+      (transpose_iindex_right op2 op3 i2 i3)
+    = normalize_iindex_right op2 op1
+        (transpose_iindex_right op2 op3 i2 i3)
+        (transpose_iindex_right op1 op3
+          (transpose_iindex_right op1 op2 i1 i2) i3).
+Proof.
+  intros i1 i2 i3 (*Hirr1 Hirr2 Hirr3*).
+  remember op1 as oper1.
+  remember op2 as oper2.
+  remember op3 as oper3.
+  destruct oper1, oper2, oper3; cbn in *;
+    case_order i1 i2;
+      case_order i2 i3; try easy;
+        case_order i1 i3; try easy.
+  - case_order i3 (pred i1).
+  - case_order i2 (pred i1).
+  - case_order i2 (S i1).
+    
+  - case_order i1 (pred i3).
+  - case_order i2 (pred i3).
+  - case_order i1 (pred i3).
+  - case_order i1 (pred i3).
+Qed.
 
 (* Given a sequence of n operations, the operational transforms
    essentially give us transpositions σᵢ which swap the ith and (i+1)th
@@ -481,6 +769,14 @@ Lemma simpl_unshift_shift_index_shift_above_index i j :
   unshift_index (shift_index i j) (shift_above_index j i) = i.
 Proof. case_order i j. Qed.
 
+     shift (shift n m) (unshift m n) = n
+     unshift (shift_above n m) (shift m n) = n
+     shift_above (unshift n m) (unshift m n) = n
+     unshift (unshift n m) (shift m n) = n
+     shift (unshift n m) (unshift m n) = n
+     unshift (shift n m) (shift_above m n) = n
+
+
 (* Unshift is right inverse of shift *)
 Lemma simpl_shift_index_unshift_index i j :
   unshift_index i (shift_index i j) = j.
@@ -501,77 +797,6 @@ Hint Rewrite simpl_shift_shift_index_unshift_index
 
 Hint Rewrite simpl_unshift_index_shift_index
   using congruence : simpl_indexs.
-
-(* Unfolding derived operations *)
-
-Lemma unfold_move_iindex {T M} i j (f : iindex T M) :
-  move_iindex i j f =
-  insert_iindex i (get_iindex j f) (delete_iindex j f).
-Proof. easy. Qed.
-
-Hint Rewrite @unfold_move_iindex : unfold_iindexs.
-
-(* Folding derived operations *)
-
-Lemma fold_move_iindex {T M} i j (f : iindex T M) :
-  insert_iindex i (get_iindex j f) (delete_iindex j f)
-  = move_iindex i j f.
-Proof. easy. Qed.
-
-Hint Rewrite @fold_move_iindex : fold_iindexs.
-
-(* Simplify [iindex] terms by unfolding, simplifying and folding *)
-Ltac simpl_iindexs :=
-  autorewrite with unfold_iindexs;
-  autorewrite with simpl_indexs simpl_iindexs;
-  repeat progress
-    (cbn;
-     try (rewrite_strat topdown (hints simpl_indexs));
-     try (rewrite_strat topdown (hints simpl_iindexs)));
-  autorewrite with fold_iindexs.
-
-Ltac simpl_iindexs_eqn :=
-  autorewrite with unfold_iindexs;
-  autorewrite with simpl_indexs simpl_iindexs;
-  repeat progress
-    (cbn;
-     try (rewrite_strat topdown (hints simpl_indexs));
-     try (rewrite_strat topdown (hints simpl_iindexs));
-     try (rewrite_strat topdown (hints simpl_iindexs_eqn)));
-  autorewrite with fold_iindexs.
-
-Ltac simpl_iindexs_pointwise :=
-  autorewrite with unfold_iindexs;
-  autorewrite with simpl_indexs simpl_iindexs_pointwise;
-  repeat progress
-    (cbn;
-     try (rewrite_strat topdown (hints simpl_indexs));
-     try (rewrite_strat topdown (hints simpl_iindexs_pointwise)));
-  autorewrite with fold_iindexs.
-
-Ltac simpl_iindexs_pointwise_eqn :=
-  autorewrite with unfold_iindexs;
-  autorewrite with simpl_indexs simpl_iindexs_pointwise;
-  repeat progress
-    (cbn;
-     try (rewrite_strat topdown (hints simpl_indexs));
-     try (rewrite_strat topdown (hints simpl_iindexs_pointwise));
-     try (rewrite_strat topdown (hints simpl_iindexs_pointwise_eqn)));
-  autorewrite with fold_iindexs.
-
-(* Useful lemmas about shifting *)
-
-Lemma shift_index_neq i j :
-  shift_index i j <> i.
-Proof.
-  case_order i j; omega.
-Qed.
-
-Lemma shift_above_index_neq_shift_index i j :
-  shift_above_index i j <> shift_index j i.
-Proof.
-  case_order i j; omega.
-Qed.
 
 (* Commuting [iindex] operations *)
 
